## 求证莫比乌斯反演

设$F(n)=\sum_{d|n}{f(d)}$ 求证$f(n)=\sum_{d|n}{\mu(d)F(\frac{n}{d})}$

​    $F(n)=\sum_{n|d}{f(d)}$ 求证$f(n)=\sum_{n|d}{\mu(\frac{d}{n})F(d)}$



性质：1、$n>1$且$n$为正整数，则有：

​		       	   $\sum_{d|n}\mu(d)=0$

​	         如果有$n=1$则式为1（$\mu(1)=1$）

​	    2、$∀n\in N^*$均有

​                           $\sum_{d|n}{\frac{\mu(d)}{d}}=\frac{\varphi(n)}{n}$



证明：∵$\sum_{d|n}{\mu(d)F(\frac{n}{d})=\sum_{d|n}{\mu(d)}\sum_{d'|\frac{n}{d}}f(d')}$

​	      令$\frac{n}{d}=kd'$，那么$d=\frac{n}{kd'}$，所以有$d|\frac{n}{d'}$

​	      而每个$f(d')$一定会和每一个$\mu(d)$乘一次，所以：

​	      $\sum_{d|n}{\mu(d)F(\frac{n}{d})}=\sum_{d'|n}{f(d')}\sum_{d|\frac{n}{d'}}{\mu(d)}$

​	      再看性质1：

​	      $\sum_{d|n}{\mu(d)F(\frac{n}{d})}=\sum_{d'|n}{f(d')}\sum_{d|\frac{n}{d'}}{\mu(d)}=f(n)$

​	      这是因为只有$d'=n$时$\mu$才有值为1，否则$\mu$无值，即为$f(n)$。